Finished first version of tr_trm in TrLowLevel.

TrLowLevel.v
@@ -22,17 +22,14 @@ Require Export Semantics LibSet LibMap LibList TLCbuffer Typing.
 
 (* ---------------------------------------------------------------------- *)
 
-
-
-
 (** Transformation of states: m ~ |m| *)
 
-Inductive tr_state (C:typdefctx) (LLC:low_level_ctx) (φ:phi) : state -> state -> Prop :=
+Inductive tr_state (C:typdefctx) (LLC:ll_typdefctx) (φ:phi) : state -> state -> Prop :=
   | tr_state_intro : forall m m',
       dom m = dom m' ->
       (forall l lw T,
         l \indom m ->
-            typing_val C φ m[l] T
+            typing_val C LLC φ m[l] T
         /\  tr_ll_val C LLC T m[l] lw
         /\  m'[l] = val_words lw) ->
       tr_state C LLC φ m m'.
@@ -40,45 +37,47 @@ Inductive tr_state (C:typdefctx) (LLC:low_level_ctx) (φ:phi) : state -> state -
 (* ---------------------------------------------------------------------- *)
 (* Transformation of a term from high-level to low-level. This is how the code is transformed. *)
 
-Inductive tr_ptrs (C:typdefctx) (LLC:low_level_ctx) : val -> val -> Prop :=
-  | tr_ptrs_unit :
-      tr_ptrs C LLC (val_basic val_unit) (val_basic val_unit)
-  | tr_ptrs_bool : forall b,
-      tr_ptrs C LLC (val_basic (val_bool b)) (val_basic (val_bool b))
-  | tr_ptrs_int : forall i,
-      tr_ptrs C LLC (val_basic (val_int i)) (val_basic (val_int i))
-  | tr_ptrs_double : forall d,
-      tr_ptrs C LLC (val_basic (val_double d)) (val_basic (val_double d))
-  | tr_ptrs_abstract_ptr : forall π l o,
+Inductive tr_val (C:typdefctx) (LLC:ll_typdefctx) : val -> val -> Prop :=
+  | tr_val_error :
+      tr_val C LLC val_error val_error
+  | tr_val_unit :
+      tr_val C LLC val_unit val_unit
+  | tr_val_bool : forall b,
+      tr_val C LLC (val_bool b) (val_bool b)
+  | tr_val_int : forall i,
+      tr_val C LLC (val_int i) (val_int i)
+  | tr_val_double : forall d,
+      tr_val C LLC (val_double d) (val_double d)
+  | tr_val_abstract_ptr : forall π l o,
       tr_ll_accesses C LLC π o ->
-      tr_ptrs C LLC (val_basic (val_abstract_ptr l π)) (val_basic (val_concrete_ptr l o))
-  | tr_ptrs_array : forall T a a',
-      List.Forall2 (tr_ptrs C LLC) a a' ->
-      tr_ptrs C LLC (val_array T a) (val_array T a')
-  | tr_ptrs_struct : forall Tv s s',
+      tr_val C LLC (val_abstract_ptr l π) (val_concrete_ptr l o)
+  | tr_val_array : forall T a a',
+      List.Forall2 (tr_val C LLC) a a' ->
+      tr_val C LLC (val_array T a) (val_array T a')
+  | tr_val_struct : forall Tv s s',
       dom s = dom s' ->
       (forall f,
         index s f ->
-        tr_ptrs C LLC s[f] s'[f]) ->
-      tr_ptrs C LLC (val_struct (typ_var Tv) s) (val_struct (typ_var Tv) s').
+        tr_val C LLC s[f] s'[f]) ->
+      tr_val C LLC (val_struct (typ_var Tv) s) (val_struct (typ_var Tv) s').
 
 (** Transformation of stacks: S ~ |S| *)
 
-Inductive tr_stack_item (C:typdefctx) (LLC:low_level_ctx) : (var * val) -> (var * val) -> Prop :=
+Inductive tr_stack_item (C:typdefctx) (LLC:ll_typdefctx) : (var * val) -> (var * val) -> Prop :=
   | tr_stack_item_intro : forall x v v',
-      tr_ptrs C LLC v v' -> 
+      tr_val C LLC v v' -> 
       tr_stack_item C LLC (x, v) (x, v').
 
-Inductive tr_stack (C:typdefctx) (LLC:low_level_ctx) : stack -> stack -> Prop :=
+Inductive tr_stack (C:typdefctx) (LLC:ll_typdefctx) : stack -> stack -> Prop :=
   | tr_stack_intro : forall S S',
       LibList.Forall2 (tr_stack_item C LLC) S S' ->
       tr_stack C LLC S S'.
 
 (** Transformation of terms: t ~ |t| *)
 
-Inductive tr_trm (C:typdefctx) (LLC:low_level_ctx) : trm -> trm -> Prop :=
+Inductive tr_trm (C:typdefctx) (LLC:ll_typdefctx) : trm -> trm -> Prop :=
   | tr_trm_val : forall v v',
-      tr_ptrs C LLC v v' ->
+      tr_val C LLC v v' ->
       tr_trm C LLC (trm_val v) (trm_val v')
   | tr_trm_var : forall x,
       tr_trm C LLC (trm_var x) (trm_var x)
@@ -100,26 +99,49 @@ Inductive tr_trm (C:typdefctx) (LLC:low_level_ctx) : trm -> trm -> Prop :=
       tr_trm C LLC (trm_app (prim_get T) (t1::nil)) (trm_app (prim_ll_get T) (t1'::nil))
   | tr_trm_set : forall t1 t2 T t1' t2',
       tr_trm C LLC t1 t1' ->
-      tr_trm C LLC (trm_app (prim_set T) (t1::t2::nil)) (trm_app (prim_ll_set T) (t1'::t2'::nil)).
-(*| tr_trm_new : 
-  | tr_trm_new_array :
-  | tr_trm_struct_access :
-  | tr_trm_array_access :
-  | tr_trm_struct_get :
-  | tr_trm_array_get :*)
+      tr_trm C LLC (trm_app (prim_set T) (t1::t2::nil)) (trm_app (prim_ll_set T) (t1'::t2'::nil))
+  | tr_trm_new : forall T,
+      tr_trm C LLC (trm_app (prim_new T) nil) (trm_app (prim_ll_new T) nil)
+ (*| tr_trm_new_array :
+      TODO: prim_new_array is needed here. *)
+  | tr_trm_struct_access : forall Tfs t1' o Tv f t1 tr,
+      Tv \indom C ->
+      typing_struct C (typ_var Tv) Tfs ->
+      f \indom Tfs ->
+      o = (fields_offsets LLC)[Tv][f] ->
+      tr_trm C LLC t1 t1' ->
+      tr = trm_app (prim_ll_access Tfs[f]) (t1'::(trm_val (val_int o))::nil) ->
+      tr_trm C LLC (trm_app (prim_struct_access (typ_var Tv) f) (t1::nil)) tr
+  | tr_trm_array_access : forall os t2' n tr T' t1' toff T t1 t2,
+      typing_array C T T' os ->
+      typ_size (typvar_sizes LLC) T' n ->
+      tr_trm C LLC t1 t1' ->
+      tr_trm C LLC t2 t2' ->
+      toff = trm_app (prim_binop binop_mul) (t2'::(trm_val (val_int n))::nil) ->
+      tr = trm_app (prim_ll_access T') (t1'::toff::nil) ->
+      tr_trm C LLC (trm_app (prim_array_access T) (t1::t2::nil)) tr
+  | tr_trm_struct_get : forall t1 T f t1',
+      tr_trm C LLC t1 t1' ->
+      tr_trm C LLC (trm_app (prim_struct_get T f) (t1::nil)) (trm_app (prim_struct_get T f) (t1'::nil))
+  | tr_trm_array_get : forall t1 t2 T t1' t2',
+      tr_trm C LLC t1 t1' ->
+      tr_trm C LLC t2 t2' ->
+      tr_trm C LLC (trm_app (prim_array_get T) (t1::t2::nil)) (trm_app (prim_array_get T) (t1'::t2'::nil)).
 
 Theorem red_tr : forall m2 t m1 φ S LLC v C S' m1' t',
-  red C S m1 t m2 v ->
-  low_level_ctx_ok C LLC ->
+  red C LLC S m1 t m2 v ->
+  ll_typdefctx_ok C LLC ->
   tr_trm C LLC t t' ->
   tr_stack C LLC S S' ->
   tr_state C LLC φ m1 m1' ->
-  state_typing C φ m1 ->
+  state_typing C LLC φ m1 ->
   exists m2' v',
-      tr_ptrs C LLC v v'
+      tr_val C LLC v v'
   /\  tr_state C LLC φ m2 m2'
-  /\  red C S' m1' t' m2' v'.
+  /\  red C LLC S' m1' t' m2' v'.
 Proof.
+  introv HR Hok Ht HS Hm1 Hφ. gen φ t' S' m1'. induction HR; intros. 
+  20:{ exists m1' val_error. inverts Ht. }
 Admitted.
 
 
